Wad math and tx params

Lsc/Arithmetic.lean
@@ -1,7 +1,9 @@
 import Lsc.Lib.Wei.Syntax
+import Lsc.Lib.Wad.Syntax
 
 namespace Lsc
 
 abbrev Wei := Wei.Wei
+abbrev Wad := Wad.Wad
 
 end Lsc
