Lsc/Prelude.lean
@@ -1,6 +1,7 @@
 import Lsc.Types
 import Lsc.Arithmetic
 import Lsc.Lib.Wei
+import Lsc.Lib.Wad
 import Lsc.Lang.AST
 import Lsc.Lang.Eval
 import Lsc.Lang.Checks
