examples/interest/lakefile.lean
@@ -1,0 +1,19 @@
+import Lake
+open Lake DSL
+
+package interest where
+  version := v!"0.1.0"
+
+require lsc from "../.."
+
+lean_lib Interest where
+  srcDir := "src"
+  roots := #[`Interest]
+
+lean_lib InterestProofs where
+  srcDir := "test"
+  roots := #[`InterestProofs]
+
+lean_lib InterestTheorems where
+  srcDir := "test"
+  roots := #[`InterestTheorems]
